Lean4Lean/Theory/Typing/EnvLemmas.lean
@@ -5,22 +5,23 @@ import Lean4Lean.Theory.Typing.InductiveLemmas
 
 namespace Lean4Lean
 
-theorem VEnv.WF.ordered (H : WF ds env) : Ordered env := by
-  induction H with
-  | empty => exact .empty
-  | decl h _ ih =>
-    cases h with
-    | block h => exact .const ih (by rintro _ ⟨⟩) h
-    | «axiom» h1 h2 => exact .const ih (by rintro _ ⟨⟩; exact h1) h2
-    | @«def» env env' ci h1 h2 =>
-      refine .defeq (.const ih (by rintro _ ⟨⟩; exact h1.isType ih ⟨⟩) h2) ⟨?_, ?_⟩
-      · simp [VDefVal.toDefEq]
-        rw [← (h1.levelWF ⟨⟩).2.2.instL_id]
-        exact .const (addConst_self h2) VLevel.id_WF (by simp)
-      · exact h1.mono (addConst_le h2)
-    | «opaque» h1 h2 => exact .const ih (by rintro _ ⟨⟩; exact h1.isType ih ⟨⟩) h2
-    | «example» _ => exact ih
-    | quot h1 h2 => exact addQuot_WF ih h1 h2
-    | induct h1 h2 => exact addInduct_WF ih h1 h2
+theorem VEnv.WF.ordered : WF env → Ordered env
+  | ⟨ds, H⟩ => by
+    induction H with
+    | empty => exact .empty
+    | decl h _ ih =>
+      cases h with
+      | block h => exact .const ih (by rintro _ ⟨⟩) h
+      | «axiom» h1 h2 => exact .const ih (by rintro _ ⟨⟩; exact h1) h2
+      | @«def» env env' ci h1 h2 =>
+        refine .defeq (.const ih (by rintro _ ⟨⟩; exact h1.isType ih ⟨⟩) h2) ⟨?_, ?_⟩
+        · simp [VDefVal.toDefEq]
+          rw [← (h1.levelWF ⟨⟩).2.2.instL_id]
+          exact .const (addConst_self h2) VLevel.id_WF (by simp)
+        · exact h1.mono (addConst_le h2)
+      | «opaque» h1 h2 => exact .const ih (by rintro _ ⟨⟩; exact h1.isType ih ⟨⟩) h2
+      | «example» _ => exact ih
+      | quot h1 h2 => exact addQuot_WF ih h1 h2
+      | induct h1 h2 => exact addInduct_WF ih h1 h2
 
-instance : CoeOut (VEnv.WF ds env) env.Ordered := ⟨(·.ordered)⟩
+instance : CoeOut (VEnv.WF env) env.Ordered := ⟨(·.ordered)⟩
