Lean4Lean/Theory/Typing/UniqueTyping.lean
@@ -70,26 +70,26 @@ theorem IsDefEqU.trans (henv : Ordered env) (hΓ : OnCtx Γ (env.IsType U))
     (h1 : env.IsDefEqU U Γ e₁ e₂) (h2 : env.IsDefEqU U Γ e₂ e₃) :
     env.IsDefEqU U Γ e₁ e₃ := h1.imp fun _ h1 => let ⟨_, h2⟩ := h2; h1.trans_l henv hΓ h2
 
-theorem IsDefEqU.sort_inv (henv : VEnv.WF ds env) (hΓ : OnCtx Γ (env.IsType U))
+theorem IsDefEqU.sort_inv (henv : VEnv.WF env) (hΓ : OnCtx Γ (env.IsType U))
     (h1 : env.IsDefEqU U Γ (.sort u) (.sort v)) : u ≈ v := sorry
 
-theorem IsDefEqU.forallE_inv (henv : VEnv.WF ds env) (hΓ : OnCtx Γ (env.IsType U))
+theorem IsDefEqU.forallE_inv (henv : VEnv.WF env) (hΓ : OnCtx Γ (env.IsType U))
     (h1 : env.IsDefEqU U Γ (.forallE A B) (.forallE A' B')) :
     (∃ u, env.IsDefEq U Γ A A' (.sort u)) ∧ ∃ u, env.IsDefEq U (A::Γ) B B' (.sort u) := sorry
 
-theorem IsDefEqU.sort_forallE_inv (henv : VEnv.WF ds env) (hΓ : OnCtx Γ (env.IsType U)) :
+theorem IsDefEqU.sort_forallE_inv (henv : VEnv.WF env) (hΓ : OnCtx Γ (env.IsType U)) :
     ¬env.IsDefEqU U Γ (.sort u) (.forallE A B) := sorry
 
-variable! (henv : VEnv.WF ds env) (hΓ : OnCtx Γ' (env.IsType U)) in
+variable! (henv : VEnv.WF env) (hΓ : OnCtx Γ' (env.IsType U)) in
 theorem IsDefEqU.weakN_iff (W : Ctx.LiftN n k Γ Γ') :
     env.IsDefEqU U Γ' (e1.liftN n k) (e2.liftN n k) ↔ env.IsDefEqU U Γ e1 e2 := by
   refine ⟨fun h => have := henv; have := hΓ; sorry, fun h => h.weakN henv W⟩
 
-variable! (henv : VEnv.WF ds env) (hΓ : OnCtx Γ' (env.IsType U)) in
+variable! (henv : VEnv.WF env) (hΓ : OnCtx Γ' (env.IsType U)) in
 theorem _root_.Lean4Lean.VExpr.WF.weakN_iff (W : Ctx.LiftN n k Γ Γ') :
     VExpr.WF env U Γ' (e.liftN n k) ↔ VExpr.WF env U Γ e := IsDefEqU.weakN_iff henv hΓ W
 
-theorem IsDefEq.skips (henv : VEnv.WF ds env) (hΓ : OnCtx Γ' (env.IsType U))
+theorem IsDefEq.skips (henv : VEnv.WF env) (hΓ : OnCtx Γ' (env.IsType U))
     (W : Ctx.LiftN n k Γ Γ')
     (H : env.IsDefEq U Γ' e₁ e₂ A) (h1 : e₁.Skips n k) (h2 : e₂.Skips n k) :
     ∃ B, env.IsDefEq U Γ' e₁ e₂ B ∧ B.Skips n k := by
@@ -98,7 +98,7 @@ theorem IsDefEq.skips (henv : VEnv.WF ds env) (hΓ : OnCtx Γ' (env.IsType U))
   have ⟨_, H⟩ := (IsDefEqU.weakN_iff henv hΓ W).1 ⟨_, H⟩
   exact ⟨_, H.weakN henv W, .liftN⟩
 
-variable! (henv : VEnv.WF ds env) (hΓ' : OnCtx Γ' (env.IsType U)) (hΓ : OnCtx Γ (env.IsType U)) in
+variable! (henv : VEnv.WF env) (hΓ' : OnCtx Γ' (env.IsType U)) (hΓ : OnCtx Γ (env.IsType U)) in
 theorem IsDefEq.weakN_iff' (W : Ctx.LiftN n k Γ Γ') :
     env.IsDefEq U Γ' (e1.liftN n k) (e2.liftN n k) (A.liftN n k) ↔ env.IsDefEq U Γ e1 e2 A := by
   refine ⟨fun h => ?_, fun h => h.weakN henv W⟩
@@ -106,7 +106,7 @@ theorem IsDefEq.weakN_iff' (W : Ctx.LiftN n k Γ Γ') :
   refine IsDefEqU.defeqDF henv hΓ ?_ H
   exact (IsDefEqU.weakN_iff henv hΓ' W).1 <| (H.weakN henv W).uniqU henv hΓ' h.symm
 
-variable! (henv : VEnv.WF ds env) in
+variable! (henv : VEnv.WF env) in
 theorem _root_.Lean4Lean.OnCtx.weakN_inv
     (W : Ctx.LiftN n k Γ Γ') (H : OnCtx Γ' (env.IsType U)) : OnCtx Γ (env.IsType U) := by
   induction W with
@@ -119,27 +119,27 @@ theorem _root_.Lean4Lean.OnCtx.weakN_inv
     let ⟨H1, _, H2⟩ := H
     exact ⟨ih H1, _, (IsDefEq.weakN_iff' henv H1 (ih H1) W).1 H2⟩
 
-variable! (henv : VEnv.WF ds env) (hΓ' : OnCtx Γ' (env.IsType U)) in
+variable! (henv : VEnv.WF env) (hΓ' : OnCtx Γ' (env.IsType U)) in
 theorem IsDefEq.weakN_iff (W : Ctx.LiftN n k Γ Γ') :
     env.IsDefEq U Γ' (e1.liftN n k) (e2.liftN n k) (A.liftN n k) ↔ env.IsDefEq U Γ e1 e2 A :=
   IsDefEq.weakN_iff' henv hΓ' (hΓ'.weakN_inv henv W) W
 
-variable! (henv : VEnv.WF ds env) (hΓ' : OnCtx Γ' (env.IsType U)) in
+variable! (henv : VEnv.WF env) (hΓ' : OnCtx Γ' (env.IsType U)) in
 theorem HasType.weakN_iff (W : Ctx.LiftN n k Γ Γ') :
     env.HasType U Γ' (e.liftN n k) (A.liftN n k) ↔ env.HasType U Γ e A :=
   IsDefEq.weakN_iff henv hΓ' W
 
-variable! (henv : VEnv.WF ds env) (hΓ' : OnCtx Γ' (env.IsType U)) in
+variable! (henv : VEnv.WF env) (hΓ' : OnCtx Γ' (env.IsType U)) in
 theorem IsType.weakN_iff (W : Ctx.LiftN n k Γ Γ') :
     env.IsType U Γ' (A.liftN n k) ↔ env.IsType U Γ A :=
   exists_congr fun _ => HasType.weakN_iff henv hΓ' W (A := .sort _)
 
-variable! (henv : VEnv.WF ds env) (hΓ' : OnCtx Γ' (env.IsType U)) in
+variable! (henv : VEnv.WF env) (hΓ' : OnCtx Γ' (env.IsType U)) in
 theorem HasType.skips (W : Ctx.LiftN n k Γ Γ')
     (h1 : env.HasType U Γ' e A) (h2 : e.Skips n k) : ∃ B, env.HasType U Γ' e B ∧ B.Skips n k :=
   IsDefEq.skips henv hΓ' W h1 h2 h2
 
-variable! (henv : VEnv.WF ds env) (hΓ' : OnCtx Γ' (env.IsType U)) in
+variable! (henv : VEnv.WF env) (hΓ' : OnCtx Γ' (env.IsType U)) in
 theorem IsDefEqU.weak'_iff (W : Ctx.Lift' l Γ Γ') :
     env.IsDefEqU U Γ' (e1.lift' l) (e2.lift' l) ↔ env.IsDefEqU U Γ e1 e2 := by
   generalize e : l.depth = n
@@ -151,7 +151,7 @@ theorem IsDefEqU.weak'_iff (W : Ctx.Lift' l Γ Γ') :
     simp only [Lift.consN_skip_eq, VExpr.lift'_comp, VExpr.lift'_consN_skipN,
       weakN_iff henv hΓ' W2, ih (hΓ'.weakN_inv henv W2) W1 Lift.depth_consN]
 
-variable! (henv : VEnv.WF ds env) (hΓ' : OnCtx Γ' (env.IsType U)) in
+variable! (henv : VEnv.WF env) (hΓ' : OnCtx Γ' (env.IsType U)) in
 theorem IsDefEq.weak'_iff (W : Ctx.Lift' l Γ Γ') :
     env.IsDefEq U Γ' (e1.lift' l) (e2.lift' l) (A.lift' l) ↔ env.IsDefEq U Γ e1 e2 A := by
   generalize e : l.depth = n
@@ -163,12 +163,12 @@ theorem IsDefEq.weak'_iff (W : Ctx.Lift' l Γ Γ') :
     simp only [Lift.consN_skip_eq, VExpr.lift'_comp, VExpr.lift'_consN_skipN,
       weakN_iff henv hΓ' W2, ih (hΓ'.weakN_inv henv W2) W1 Lift.depth_consN]
 
-variable! (henv : VEnv.WF ds env) (hΓ' : OnCtx Γ' (env.IsType U)) in
+variable! (henv : VEnv.WF env) (hΓ' : OnCtx Γ' (env.IsType U)) in
 theorem HasType.weak'_iff (W : Ctx.Lift' l Γ Γ') :
     env.HasType U Γ' (e.lift' l) (A.lift' l) ↔ env.HasType U Γ e A :=
   IsDefEq.weak'_iff henv hΓ' W
 
-variable! (henv : VEnv.WF ds env) (hΓ' : OnCtx Γ' (env.IsType U)) in
+variable! (henv : VEnv.WF env) (hΓ' : OnCtx Γ' (env.IsType U)) in
 theorem IsType.weak'_iff (W : Ctx.Lift' l Γ Γ') :
     env.IsType U Γ' (e.lift' l) ↔ env.IsType U Γ e :=
   exists_congr fun _ => HasType.weak'_iff henv hΓ' W (A := .sort _)
